Wip

concordium-provider/src/auction_provider.rs
@@ -1,5 +1,5 @@
 use crate::provider::Action;
-use auction::*;
+use auction::{State as AucState, *};
 use concordium_std::{collections::BTreeMap, *};
 use core::fmt::Debug;
 use hacspec_lib::*;
@@ -34,25 +34,13 @@ pub enum AuctionState {
     Sold(AccountAddress), // winning account's address
 }
 
-/// The state of the smart contract.
-/// This is the state that will be shown when the contract is queried using
-/// `concordium-client contract show`.
 #[contract_state(contract = "auction")]
 #[derive(Debug, Serialize, SchemaType, Eq, PartialEq)]
 pub struct State {
-    /// Has the item been sold?
     auction_state: AuctionState,
-    /// The highest bid so far (stored explicitly so that bidders can quickly
-    /// see it)
     highest_bid: concordium_std::Amount,
-    /// The sold item (to be displayed to the auction participants), encoded in
-    /// ASCII
     item: Vec<u8>,
-    /// Expiration time of the auction at which bids will be closed (to be
-    /// displayed to the auction participants)
     expiry: concordium_std::Timestamp,
-    /// Keeping track of which account bid how much money
-    #[concordium(size_length = 2)]
     bids: BTreeMap<AccountAddress, concordium_std::Amount>,
 }
 
@@ -88,13 +76,12 @@ fn seq_map_to_btree_map(m: SeqMap) -> BTreeMap<AccountAddress, concordium_std::A
 }
 
 fn my_state_to_their_state(s: auction::State) -> State {
-    let auction::State (st0, st1, st2, st3, st4) = s;
     State {
-        auction_state: my_auction_state_to_their_auction_state(st0),
-        highest_bid: concordium_std::Amount { micro_gtu: st1 },
-        item: st2.native_slice().to_vec(),
-        expiry: concordium_std::Timestamp::from_timestamp_millis(st3),
-        bids: seq_map_to_btree_map(st4),
+        auction_state: my_auction_state_to_their_auction_state(s.0),
+        highest_bid: concordium_std::Amount { micro_gtu: s.1 },
+        item: s.2.native_slice().to_vec(),
+        expiry: concordium_std::Timestamp::from_timestamp_millis(s.3),
+        bids: seq_map_to_btree_map(s.4),
     }
 }
 
@@ -159,7 +146,7 @@ fn their_auction_state_to_my_auction_state(s: AuctionState) -> auction::AuctionS
 }
 
 fn btree_map_to_seq_map(m: BTreeMap<AccountAddress, concordium_std::Amount>) -> SeqMap {
-    (
+    SeqMap(
         m.keys()
             .map(|x| u8x32_to_user_address(x.0))
             .fold(PublicByteSeq::new(0_usize), |v, x| v.concat(&x)),
@@ -174,7 +161,7 @@ fn btree_map_to_seq_map(m: BTreeMap<AccountAddress, concordium_std::Amount>) -> 
 }
 
 fn their_state_to_my_state(s: &mut State) -> auction::State {
-    auction::State (
+    auction::State(
         their_auction_state_to_my_auction_state(s.auction_state.clone()),
         s.highest_bid.micro_gtu,
         Seq::from_vec(s.item.clone()),
