lib/src/struct_unfold.rs
@@ -1,15 +1,48 @@
 #[macro_export]
 macro_rules! unfold_struct {
     (
-        $vis:vis struct $struct_name:ident {
-            $($field_vis:vis $field_name:ident : $field_type:ty),*$(,)+
+        struct $struct_name:ident {
+            $($field_name:ident : $field_type:ty),*$(,)+
         }
     ) => {
-        $vis type $struct_name = ($($field_type),*);
+	#[derive(Clone)]
+        pub struct $struct_name ($(pub $field_type),*);
     };
 }
 
-// #[allow(non_camel_case_types)]
-// #[derive(Clone)]
-// $vis struct $struct_name ($($field_vis $field_type),*);
+#[macro_export]
+macro_rules! translate_field {
+    ( $fn_name:ident, $enum_name_from:ty, $enum_name_to:ty, $($rest:ident),* ) => {
+	fn $fn_name(their_ident : $enum_name_from) -> $enum_name_to {
+	    match their_ident {
+		$(<$enum_name_from>::$rest => <$enum_name_to>::$rest),*
+	    }
+	}
+    }
+}
 
+    // ($ty:ty) => {
+    // 	fn their_to_my_$ty(their_ident : $ty) -> $ty {
+    // 	    their_ident
+    // 	}
+    // },
+
+// #[macro_export]
+// macro_rules! struct_to_unfold_struct_translations {
+//     (
+// 	$unfold_struct:ident,
+//         pub struct $struct_name:ident {
+//             $($field_name:ident : $field_type:ty),*$(,)+
+//         }
+//     ) => {
+// 	$(translate_field!($field_name, $field_type)),*
+	
+//         fn their_to_my_struct (their_struct : $struct_name) -> $unfold_struct {
+// 	    $unfold_struct ($(their_struct.$field_name),*) // [their_struct.]$($field_name)+
+// 	}
+	
+//         // fn my_to_their_$struct_name (my_struct : $unfold_struct) -> $struct_name {
+// 	//     let $unfold_struct ($($field_name),*) = my_struct;
+// 	// }	
+//     };
+// }
